libcrux-ml-dsa/proofs/fstar/spec/Spec.MLDSA.Ntt.fst
@@ -1,10 +1,9 @@
  module Spec.MLDSA.Ntt
  open Core
  open FStar.Mul
-
- #set-options "--fuel 0 --ifuel 0 --z3rlimit 100"
+ open Spec.MLDSA.Math
  
- assume val mont_mul: i32 -> i32 -> i32
+ #set-options "--fuel 0 --ifuel 0 --z3rlimit 100"
 
  let ntt_step zeta (a, b) =
      let t = mont_mul b zeta in
